src/polytime/size.lean
@@ -1,0 +1,91 @@
+import encode
+
+open tencodable function tree
+variables {α β γ : Type*}
+
+class polysize (α : Type*) [tencodable α] :=
+(size : α → ℕ)
+(upper [] : ∃ p : polynomial ℕ, ∀ x, size x ≤ p.eval (encode x).num_nodes)
+(lower [] : ∃ p : polynomial ℕ, ∀ x, (encode x).num_nodes ≤ p.eval (size x))
+
+open polysize
+variables [tencodable α] [tencodable β] [tencodable γ]
+
+instance : inhabited (polysize α) :=
+⟨{ size := λ x, (encode x).num_nodes,
+  upper := ⟨polynomial.X, by simp⟩,
+  lower := ⟨polynomial.X, by simp⟩ }⟩
+
+@[simps]
+instance fintype.polysize [fintype α] : polysize α :=
+{ size := λ _, 0,
+  upper := ⟨0, λ x, zero_le'⟩,
+  lower := ⟨polynomial.C ((@finset.univ α _).sup (λ x, (encode x).num_nodes)), 
+    λ x, by { simp, exact finset.le_sup (finset.mem_univ x), }⟩ }
+
+instance [polysize α] [polysize β] : polysize (α × β) :=
+begin
+  refine_struct { size := λ x : α × β, size x.1 + size x.2 },
+  { cases upper α with p hp, cases upper β with q hq,
+    use p + q, rintro ⟨x₁, x₂⟩,
+    rw polynomial.eval_add,
+    refine add_le_add ((hp _).trans $ p.eval_mono _) ((hq _).trans $ q.eval_mono _);
+    simp [encode]; linarith only, },
+  cases lower α with p hp, cases lower β with q hq,
+  use p + q + 1, rintro ⟨x₁, x₂⟩,
+  simp only [encode, num_nodes, polynomial.eval_add, polynomial.eval_one, add_le_add_iff_right],
+  exact add_le_add ((hp _).trans $ p.eval_mono le_self_add)
+    ((hq _).trans $ q.eval_mono le_add_self),
+end
+
+@[simp] lemma polysize.prod_size [polysize α] [polysize β]
+  (x : α) (y : β) : size (x, y) = size x + size y := rfl
+
+instance : polysize ℕ := default
+instance : polysize (tree unit) := default
+
+@[simp] lemma polysize_unary_nat (n : ℕ) : size n = n :=
+by simp [polysize.size]
+
+@[simp] lemma polysize_tree_unit (x : tree unit) : size x = x.num_nodes := rfl
+
+def polysize_uniform [polysize α] [polysize β] (f : α → β → β) : Prop :=
+∃ (p : polynomial ℕ), ∀ x y, size (f x y) ≤ size y + p.eval (size x)
+
+theorem polysize_uniform.iterate [polysize α] [polysize β] {f : α → β → β} {n : α → ℕ}
+  (hf : polysize_uniform f) (hn : ∃ p : polynomial ℕ, ∀ x, n x ≤ p.eval (size x)) :
+    ∃ p : mv_polynomial (fin 2) ℕ, ∀ x y (m ≤ n x), size ((f x)^[m] y) ≤ mv_polynomial.eval ![size x, size y] p :=
+begin
+  cases hn with p hn, cases hf with q hf,
+  use (mv_polynomial.X 1 + (polynomial.to_mv 0 p) * (polynomial.to_mv 0 q) : mv_polynomial (fin 2) ℕ),
+  intros x y m hm, specialize hn x,
+  have : ∀ n : ℕ, size ((f x)^[n] y) ≤ size y + n * (q.eval $ size x),
+  { intro n, induction n with n ih, 
+    { simp, },
+    rw [iterate_succ_apply', nat.succ_mul, ← add_assoc],
+    refine (hf x _).trans _,
+    simpa using ih, },
+  refine (this $ m).trans _,
+  simp, mono, exacts [hm.trans hn, zero_le'],
+end
+
+def polysize_uniform' {β : α → Type*} [∀ x, tencodable (β x)] [polysize α] [∀ x, polysize (β x)] [polysize γ]
+  (f : ∀ x, β x → γ) : Prop :=
+∃ (p : polynomial ℕ), ∀ x y, size (f x y) ≤ size y + p.eval (size x)
+
+theorem polysize_uniform'.iterate [polysize α] [polysize β] {f : α → β → β} {n : α → ℕ}
+  (hf : polysize_uniform' f) (hn : ∃ p : polynomial ℕ, ∀ x, n x ≤ p.eval (size x)) :
+    ∃ p : mv_polynomial (fin 2) ℕ, ∀ x y (m ≤ n x), size ((f x)^[m] y) ≤ mv_polynomial.eval ![size x, size y] p :=
+begin
+  cases hn with p hn, cases hf with q hf,
+  use (mv_polynomial.X 1 + (polynomial.to_mv 0 p) * (polynomial.to_mv 0 q) : mv_polynomial (fin 2) ℕ),
+  intros x y m hm, specialize hn x,
+  have : ∀ n : ℕ, size ((f x)^[n] y) ≤ size y + n * (q.eval $ size x),
+  { intro n, induction n with n ih, 
+    { simp, },
+    rw [iterate_succ_apply', nat.succ_mul, ← add_assoc],
+    refine (hf x _).trans _,
+    simpa using ih, },
+  refine (this $ m).trans _,
+  simp, mono, exacts [hm.trans hn, zero_le'],
+end
